

1.8 Free Lie algebras

Today, all modules and algebras will be over k .

1.8.1 Free magmas

Definition 1.8.1

A set with a map $M \times M \rightarrow M$ is called a *magma*.

Let X be a set and by induction define $X_1 = X$,

$$X_n = \bigsqcup_{p+q=n} X_p \times X_q.$$

Let $M_X = \bigsqcup_{n=1}^{\infty} X_n$, and define

$$M_X \times M_X \rightarrow M_X$$

by

$$X_p \times X_q \hookrightarrow X_{p+q}$$

where \hookrightarrow denotes the canonical inclusion from the definition of X_n . We call M_X the *free magma* on X . An element of M_X is called a non-associative word on W . If $w \in X_n$, then its length is $\ell(w) = n$. The free magma enjoys the following universal property:

Proposition 1.8.2

Let N be a magma and $f: X \rightarrow N$ a map. Then there exists a unique magma homomorphism $F: M_X \rightarrow N$ such that $f = F \circ \iota$, where $\iota: X = X_1 \hookrightarrow M_X$ is the canonical inclusion.

Proof. Define F inductively by $F(u, v) = F(u) \cdot F(v)$ if $u, v \in X_p \times X_q$. □

1.8.2 Free algebras

Let A_X be the k -algebra of M_X . Concretely, each $\alpha \in A_X$ is a finite sum $\alpha = \sum_{m \in M_X} c_m m$ for $c_m \in k$, and multiplication in A_X is a linear extension of multiplication in M_X . We call A_X the *free algebra* on X . It enjoys a similar universal property:

Proposition 1.8.3

Let B be a k -algebra and $f: X \rightarrow B$ a map. Then there exists a unique k -algebra homomorphism $F: A_X \rightarrow B$ such that $f = F \circ \iota$.

Proof. By the universal property of the free magma, we have a magma homomorphism $f': M_X \rightarrow B$ which extends f . Then extend f' linearly to a k -algebra homomorphism $F: A_X \rightarrow B$. □

Remark 1.8.4. A_X admits a natural grading by longest word length.

1.8.3 Free Lie algebras

Let $I \subset A_X$ be the ideal generated by the elements aa for $a \in A_X$ and $J(a, b, c)$, where $a, b, c \in A_X$ and J denotes the Jacobi product.

We call $L_X := A_X/I$ the *free Lie algebra* on X

Proposition 1.8.5

If $f: X \rightarrow X'$ is any map, then there exists a unique map $F: L_X \rightarrow L_{X'}$ which restricts to f .

Proof. L_X has basis $\{e_x\}_{x \in X}$, so we define $F(e_x) = e_{f(x)}$. Note that this is functorial. \square

Corollary 1.8.6

Let $(X_\alpha, i_\alpha^\beta)$ be a directed system and $X = \varinjlim_\alpha X_\alpha$. Then

$$\varinjlim L_{X_\alpha} \cong L_X.$$

Proof. Let $i_\alpha: X_\alpha \rightarrow X$ be the canonical inclusions. By the previous proposition, we get $I_\alpha: L_{X_\alpha} \rightarrow L_X$ which is functorial so $L_X = \varinjlim L_{X_\alpha}$. \square

Proposition 1.8.7

If $k \subset k'$ then $L_X(k') = L_X(k) \otimes_k k'$.

Proof. We have a natural isomorphism $e_x \otimes \lambda \mapsto \lambda e_x$. \square

Proposition 1.8.8

I is a graded ideal of A_X , so L_X has a natural grading.

Proof. Let I^\sharp be the ideal of $a \in A_X$ such that every homogeneous component of a belongs to I . Then $I^\sharp \subset I$. Conversely if $x = \sum x_n \in A_X$ then

$$x^2 = \sum x_n^2 + \sum_{n < m} (x_n x_m + x_m x_n),$$

but $x_n^2 \in I$ and

$$x_n x_m + x_m x_n = (x_n + x_m)^2 - x_n^2 - x_m^2 \in I,$$

so $x^2 \in I^\sharp$. Likewise

$$J(x, y, z) = \sum_{\ell, m, n} J(x_\ell, y_m, z_n) \in I^\sharp,$$

so $I^\sharp = I$. \square

Proposition 1.8.9

L_X^1 has basis X and L_X^2 has basis $\{[x, y]\}_{x < y}$ where we have chosen a total order on X .

Proof. Clearly X generates L_X^1 and $[X, X]$ generates L_X^2 . Let $E = k^{(X)}$ and let $E \oplus \Lambda^2 E = \mathfrak{g}$ be the associated Lie algebra. The canonical map $X \rightarrow \mathfrak{g}$ yields a Lie homomorphism $L_X \rightarrow \mathfrak{g}$, and $L_X^1 \oplus L_X^2 \rightarrow L_X \rightarrow \mathfrak{g}$ is an isomorphism. \square

1.8.4 Free associative algebras

Let $E = k^{(X)}$ be the free k -module with basis X . Then the free associative algebra on X , denoted by Ass_X , is the tensor algebra TE .

Theorem 1.8.10

Let $\phi: L_X \rightarrow \text{Ass}_X$ and $\Phi: UL_X \rightarrow \text{Ass}_X$ be the maps induced by $X \rightarrow \text{Ass}_X$. Then

- (1) Φ is an isomorphism.
- (2) ϕ is an isomorphism onto the Lie subalgebra generated by X .
- (3) L_X and its homogeneous components are free k -modules.
- (4) If X is finite and $\#X = d$ then L_X^n is free of finite rank $\ell_d(n)$, which is determined by induction according to the formula

$$\sum_{m|n} m \ell_d(m) = d^n.$$

Proof. (1) is clear as $X \rightarrow UL_X$ gives a homomorphism $\Psi: \text{Ass}_X \rightarrow UL_X$, which is seen to be inverse to Φ .

Also, $\phi: L_X \rightarrow \text{Ass}_X$ maps into the Lie subalgebra generated by X , so it suffices to show ϕ is injective. By the Poincaré–Birkhoff–Witt theorem, if (3) L_X is free over k then (2) $L_X \rightarrow UL_X$ is injective, and under the identification of UL_X with Ass_X we have (2).

To prove (3) and (4), first assume k is a field and X is finite. Let $(\gamma_i)_{i \in I}$ be a totally ordered homogeneous basis for L_X . Let $d_i = \deg(\gamma_i)$. The PBW theorem implies that the elements

$$\gamma^e = \gamma_{i_1}^{e_1} \cdots \gamma_{i_s}^{e_s} \quad \text{for } i_1 < \cdots < i_s$$

form a basis of $UL_X \cong \text{Ass}_X$ and $\deg(\gamma^e) = \sum e_{i_j} d_{i_j}$. Let $a(n)$ be the rank of Ass_X^n . Then $a(n)$ is the number of families (e_i) such that $n = \sum e_i d_i$. Equivalently, the power series

$$A(t) = \sum a(n) t^n$$

can be written in the form

$$A(t) = \prod_{i \in I} \frac{1}{1 - t^{d_i}}$$

and the coefficient of t^n in

$$\prod_{i \in I} \frac{1}{1 - t^{d_i}} = \prod_{i \in I} (1 + t^{d_i} + t^{2d_i} + \cdots)$$

is the number of (e_i) such that $\sum e_i d_i = n$. For any $m \in \mathbb{N}$ we have that the number of $d_i = m$ in the product $\prod_{i \in I} \frac{1}{1-t^{d_i}}$ is $\ell_d(m)$ the rank of L_X^m , so

$$A(t) = \prod_{m=1}^{\infty} \frac{1}{(1-t^m)^{\ell_d(m)}}.$$

On the other hand, Ass_X is the free associative algebra on X and so the monomials $x_{i_1} \cdots x_{i_n}$ form a basis. So $a(n) = d^n$, and thus

$$\begin{aligned} A(t) &= \sum d^n t^n \\ \prod_{m=1}^{\infty} &= \frac{1}{1-dt} \\ \sum_{m, \nu} \frac{1}{\nu} \ell_d(m) t^{m\nu} &= \sum_{n=1}^{\infty} \frac{1}{n} d^n t^n \\ \frac{1}{n} d^n &= \sum_{m\nu=n} \frac{1}{\nu} \ell_d(m) \\ d^n &= \sum_{m|n} m \ell_d(m), \end{aligned}$$

proving (4).

Secondly, assume $k = \mathbb{Z}$ and X is finite. It is a fact from the structure theorem of abelian groups that if E is a finitely-generated \mathbb{Z} -module and $\dim_{\mathbb{F}_p}(E \otimes_{\mathbb{Z}} \mathbb{F}_p)$ is independent of p , then E is a free \mathbb{Z} -module with rank $\dim_{\mathbb{F}_p}(E \otimes_{\mathbb{Z}} \mathbb{F}_p)$. Now since $L_X^n(\mathbb{Z}) \otimes_{\mathbb{Z}} \mathbb{F}_p$ and $\dim(L_X^n(\mathbb{F}_p)) = \ell_d(n)$ is independent of p , L_X^n is a free \mathbb{Z} -module of rank $\ell_d(n)$.

Now for $k = \mathbb{Z}$ and dropping the finiteness assumption on X , let (Y_α) be the finite subsets of X , so that $X = \varinjlim_{\alpha} Y_\alpha$. We first prove (2). By the previous case

$$\phi_\alpha: L_{Y_\alpha} \rightarrow \text{Ass}_{Y_\alpha}$$

is injective. Now $\phi = \varinjlim_{\alpha} \phi_\alpha$ is injective as the colimit of injective maps, proving (2). Then (2) implies that L_X and L_X^n are \mathbb{Z} -submodules of Ass_X , which is free, so L_X and L_X^n are free.

Finally, the result for arbitrary k follows from the equality

$$L_X^n(k) = L_X^n(\mathbb{Z}) \otimes_{\mathbb{Z}} k.$$

This shows L_X^k is free (3), which implies (2). Also $\text{rank } L_X^n(k) = \text{rank } L_X^n(\mathbb{Z})$ so we have (4) when X is finite. \square

1.8.5 P. Hall families

Definition 1.8.11

Let X be a set. A *P. Hall family* in M_X is a totally ordered subset $H \subset M_X$ such that

- (i) $X \subset H$.
- (ii) If $u, v \in H$ with $\ell(u) < \ell(v)$ then $u < v$.
- (iii) Let $u \in M_X \setminus X$ and write $u = vw$. Then $u \in H$ if and only if (a) $v, w \in H$ and $v < w$,

and (b) either $w \in X$ or $w = w'w''$ with $w', w'' \in H$ and $w' \leq w''$.

Proposition 1.8.12

Every set admits a P. Hall family.

Proof. By induction, we define $H^n = H \cap X_n$. Let $H^1 = X$, and let X be totally ordered. If H^1, \dots, H^{n-1} are defined and totally ordered so that (i), (ii), (iii) hold for elements of length $\leq n-1$, then H^n is defined by (iii): we order H^n and put $u < v$ if $u \in H^i$ and $v \in H^n$. By induction, $H = \bigcup H^n$ is a P. Hall family. \square

We will not prove the following result.

Theorem 1.8.13

Let H be a P. Hall family in M_X . Then the canonical image of H is a basis of L_X .

1.8.6 Free groups

Let $k = \mathbb{Z}$. Let X be a set and F_X the free group on X . Let F_X^n be the descending central series of F_X , defined by $F_X^1 = F_X$ and $F_X^n = (F_X, F_X^{n-1})$.

The associated graded group

$$\text{gr } F_X = \sum_{n=1}^{\infty} \text{gr}_n F_X$$

where

$$\text{gr}_n F_X = F_X^n / F_X^{n+1}$$

is a Lie algebra; in particular $\text{gr}_1 F_X = F_X / (F_X, F_X)$ is the free abelian group on X .

Theorem 1.8.14

The canonical map $X \rightarrow \text{gr}_1 F_X$ induces a Lie isomorphism

$$\phi_1: L_1 \xrightarrow{\sim} \text{gr } F_X.$$

Corollary 1.8.15

The groups $\text{gr}_n F_X$ are free \mathbb{Z} -modules. If X is finite with $\#X = d$, then $\text{rank } \text{gr}_n F_X = \ell_d(n)$.

We define the completion $\hat{\text{Ass}}_X$ of Ass_X to be the product $\prod_{n=0}^{\infty} \text{Ass}_X^n$. An element $f \in \hat{\text{Ass}}_X$ is

represented by a formal series $f = \sum_{n=0}^{\infty} f_n$ with $f_n \in \text{Ass}_X^n$. We have a natural homomorphism

$$\begin{aligned} \theta: F_X &\longrightarrow \hat{\text{Ass}}_X^* \\ x &\longmapsto 1 + x. \end{aligned}$$

Let

$$\hat{\mathfrak{m}}^n = \left\{ \sum_{m=0}^{\infty} f_m \in \hat{\text{Ass}}_X : f_0 = f_1 = \cdots = f_{n-1} = 0 \right\},$$

and let $'F_X^n = \theta^{-1}(1 + \hat{\mathfrak{m}}^n)$. Then $g \in F_X$ is in $'F_X^n$ if and only if

$$\theta(g) = 1 + \sum_{m \geq n} \psi_m.$$

Theorem 1.8.16

$$'F_X^n = F_X^n.$$

Proof of Theorem 1.8.14 and Theorem 1.8.16. It is clear that ϕ_1 is surjective.

We claim that $'F_X^n$ is a filtration of F_X . It suffices to show

$$('F_X^m, 'F_X^p) \subset 'F_X^{m+p}.$$

Indeed, pick $g \in 'F_X^m$, $h \in 'F_X^p$ with $\theta(g) = 1 + G$ for $G \in \hat{\mathfrak{m}}^m$, $\theta(h) = 1 + H$ for $H \in \hat{\mathfrak{m}}^p$. Then

$$\begin{aligned} gh &= hg(g, h), \theta(gh) &= 1 + G + H + GH, \\ \theta(hg) &= 1 + G + H + HG. \end{aligned}$$

Since θ is a homomorphism we get $\theta(gh) = \theta(hg)\theta((g, h))$, so

$$\theta((g, h)) = 1 + (GH - HG) + \text{higher terms}.$$

Hence $(g, h) \in 'F_X^{m+p}$.

Now there is a natural map $\eta: ' \text{gr } F_X \rightarrow \text{Ass}_X$: given $\xi \in ' \text{gr}_n F_X$ let $g \in 'F_X^n$ be a representative and let

$$\theta(g) = 1 + G_n + G_{n+1} + \cdots,$$

where $G_p \in \text{Ass}_X^p$. Define

$$\eta(\xi) = G_n.$$

This clearly doesn't depend on g , and the above equation for $\theta((g, h))$ shows that η is a Lie homomorphism.

Now since $'F_X^n$ is a filtration we automatically have $F_X^n \subset 'F_X^n$, which yields a homomorphism $\psi: \text{gr } F_X \rightarrow ' \text{gr } F_X$. Consider the composition

$$L_X \xrightarrow{\phi_1} \text{gr } F_X \xrightarrow{\psi} ' \text{gr } F_X \xrightarrow{\eta} \text{Ass}_X,$$

where ϕ_1 is surjective and η is injective. This composition coincides with the map $\phi: L_X \rightarrow \text{Ass}_X$ we saw earlier, which is injective. Hence ϕ_1 is injective, proving Theorem 1.8.14. This implies ψ is injective. By induction, we claim that $F_X^n = 'F_X^n$. For $n = 1$ this is by definition, and if $n > 1$ then

$$F_X^n \subset 'F_X^n \subset F_X^{n-1} \subset 'F_X^{n-1},$$

and the injection

$$\text{gr}_{n-1} F_X \rightarrow ' \text{gr}_{n-1} F_X$$

is the canonical map

$$F_X^{n-1} / F_X^n \rightarrow F_X^{n-1} / 'F_X^n,$$

so $F_X^n = 'F_X^n$. □

1.8.7 The Campbell–Hausdorff formula

In this section let k be a \mathbb{Q} -algebra, for example a field of characteristic 0.

Theorem 1.8.17

Let X be a set. Then the free Lie algebra L_X is the set of primitive elements of Ass_X .

Proof. This follows from the fact that the analogous result about the universal enveloping algebra under the identification $\text{Ass}_X \cong UL_X$. \square

As with the associative algebra, define the completion of L_X by

$$\hat{L}_X = \prod_{n=0}^{\infty} L_X^n$$

and define the *completed tensor product*

$$\hat{\text{Ass}}_X \hat{\otimes} \hat{\text{Ass}}_X = \prod_{p,q} \text{Ass}_X^p \otimes \text{Ass}_X^q.$$

The diagonal $\Delta: \text{Ass}_X \rightarrow \text{Ass}_X \otimes \text{Ass}_X$ thus extends to

$$\Delta: \hat{\text{Ass}}_X \rightarrow \hat{\text{Ass}}_X \hat{\otimes} \hat{\text{Ass}}_X,$$

and the above theorem about primitive elements remains true when we pass to completions. Let $\hat{\mathfrak{m}} \subset \hat{\text{Ass}}_X$ be the ideal generated by X as before. Define

$$\begin{aligned} \exp: \hat{\mathfrak{m}} &\longrightarrow 1 + \hat{\mathfrak{m}} \\ x &\longmapsto \sum \frac{x^n}{n!}, \\ \log: 1 + \hat{\mathfrak{m}} &\longrightarrow \hat{\mathfrak{m}} \\ 1 + x &\longmapsto \sum_{n=1}^{\infty} (-1)^{n+1} \frac{x^n}{n}. \end{aligned}$$

Theorem 1.8.18

$\exp \circ \log = \text{id}$ and $\log \circ \exp = \text{id}$.

Proof. Let $y \in \hat{\mathfrak{m}}$, we show that $\exp(\log(1 + y)) = 1 + y$. For any indeterminate T , the formula

$$\exp(\log(1 + T)) = 1 + T$$

is true in $\mathbb{Q}[[T]]$. But $y \in \hat{\mathfrak{m}}$ so there exists a well-defined and continuous homomorphism $f: \mathbb{Q}[[T]] \rightarrow \hat{\text{Ass}}_X$ sending T to y , so we are done. The other formula is similar. \square

Corollary 1.8.19

\exp is a bijection of the set of primitive elements in $\hat{\mathfrak{m}}$ onto the set of $\beta \in 1 + \hat{\mathfrak{m}}$ with $\Delta\beta = \beta \otimes \beta$.

Proof. Let $\alpha \in \hat{\mathfrak{m}}$ and $\beta \in e^\alpha$. Since Δ commutes with \exp and $\alpha \otimes 1$ commutes with $1 \otimes \alpha$,

$$\Delta\beta = \Delta e^\alpha = e^{\Delta\alpha} = e^{\alpha \otimes 1 + 1 \otimes \alpha} = e^{\alpha \otimes 1} e^{1 \otimes \alpha} = (\beta \otimes 1)(1 \otimes \beta) = \beta \otimes \beta.$$

□

Now for our second big theorem:

Theorem 1.8.20 (Campbell–Hausdorff)

Let $X = \{x, y\}$ where $x \neq y$. Then $e^x e^y = e^z$ with $z \in \hat{L}_X$.

Proof. Since $e^x, e^y \in 1 + \hat{\mathfrak{m}}$ we have $e^x e^y \in 1 + \hat{\mathfrak{m}}$. Since \exp is a bijection, there exists a unique $z \in \hat{\mathfrak{m}}$ with $e^z = e^x e^y$. In particular

$$\begin{aligned} \Delta e^z &= \Delta(e^x e^y) \\ &= \Delta(e^x) \Delta(e^y) \\ &= (e^x \otimes e^x)(e^y \otimes e^y) \\ &= e^z \otimes e^z. \end{aligned}$$

By the previous proposition this implies z is a primitive element, and by the correspondence between primitive elements of Ass_X and \hat{L}_X , we have $z \in \hat{L}_X$. □

If X is arbitrary and $z(x, y)$ is the element of $\hat{L}_{\{x, y\}} \subset \hat{L}_X$ such that $e^x e^y = e^{z(x, y)}$, then write

$$z(x, y) = \sum_{n=1}^{\infty} z_n(x, y)$$

for $z_n(x, y) \in L_X^n$. Explicitly, we may compute the first few homogeneous components?

$$\begin{aligned} z_1(x, y) &= x + y \\ z_2(x, y) &= \frac{1}{2}[x, y] \\ z_3(x, y) &= \frac{1}{12}[x, [x, y]] + \frac{1}{12}[y, [y, x]]. \end{aligned}$$

It is also clear that

$$\begin{aligned} z(x, 0) &= x \\ z(0, y) &= y \\ z(z(w, x), y) &= z(w, z(x, y)). \end{aligned}$$